Simulation convention cleanup for locset-style passes

backend/Conventions.v
@@ -19,6 +19,7 @@ Require Import Values.
 Require Import Memory.
 Require Import LanguageInterface.
 Require Import Locations.
+Require Import CKLR.
 Require Export Conventions1.
 
 (** The processor-dependent and EABI-dependent definitions are in
@@ -189,6 +190,8 @@ Canonical Structure li_locset: language_interface :=
 
 (** * Calling convention *)
 
+(** ** C-style to locset-style *)
+
 (** We first define the calling convention between C and locset
   languages, which relates the C-level argument list to the contents
   of the locations. The Kripke world keeps track of the signature and
@@ -196,42 +199,50 @@ Canonical Structure li_locset: language_interface :=
   interpreted in the correct way and the preservation of callee-save
   registers can be enforced. *)
 
-Inductive cc_alloc_mq: signature * Locmap.t -> c_query -> locset_query -> Prop :=
-  cc_alloc_mq_intro vf sg args rs m:
+Inductive cc_c_locset_mq: signature * Locmap.t -> c_query -> locset_query -> Prop :=
+  cc_c_locset_mq_intro vf sg args rs m:
     args = (map (fun p => Locmap.getpair p rs) (loc_arguments sg)) ->
-    cc_alloc_mq (sg, rs) (cq vf sg args m) (lq vf sg rs m).
+    cc_c_locset_mq (sg, rs) (cq vf sg args m) (lq vf sg rs m).
 
-Inductive cc_alloc_mr: signature * Locmap.t -> c_reply -> locset_reply -> Prop :=
-  cc_alloc_mr_intro sg rs res rs' m:
+Inductive cc_c_locset_mr: signature * Locmap.t -> c_reply -> locset_reply -> Prop :=
+  cc_c_locset_mr_intro sg rs res rs' m:
     res = (Locmap.getpair (map_rpair R (loc_result sg)) rs') ->
     agree_callee_save rs rs' ->
-    cc_alloc_mr (sg, rs) (cr res m) (lr rs' m).
+    cc_c_locset_mr (sg, rs) (cr res m) (lr rs' m).
 
-Program Definition cc_alloc: callconv li_c li_locset :=
+Program Definition cc_c_locset: callconv li_c li_locset :=
   {|
     match_senv w := eq;
-    match_query := cc_alloc_mq;
-    match_reply := cc_alloc_mr;
+    match_query := cc_c_locset_mq;
+    match_reply := cc_c_locset_mr;
   |}.
 
-(** The extension convention is used by the Tunneling proof. *)
+(** ** Locset-style CKLR convention *)
 
-Inductive cc_locset_ext_query: locset_query -> locset_query -> Prop :=
-  cc_locset_ext_query_intro vf sg ls1 ls2 m1 m2:
-    (forall l, Val.lessdef (ls1 l) (ls2 l)) ->
-    Mem.extends m1 m2 ->
-    cc_locset_ext_query (lq vf sg ls1 m1) (lq vf sg ls2 m2).
+Inductive cc_locset_query R w: locset_query -> locset_query -> Prop :=
+  cc_locset_query_intro vf1 vf2 sg ls1 ls2 m1 m2:
+    Val.inject (mi R w) vf1 vf2 ->
+    (forall l, Val.inject (mi R w) (ls1 l) (ls2 l)) ->
+    match_mem R w m1 m2 ->
+    vf1 <> Vundef ->
+    cc_locset_query R w (lq vf1 sg ls1 m1) (lq vf2 sg ls2 m2).
 
-Inductive cc_locset_ext_reply: locset_reply -> locset_reply -> Prop :=
-  cc_locset_ext_reply_intro ls1 ls2 m1 m2:
-    (forall l, Val.lessdef (ls1 l) (ls2 l)) ->
-    Mem.extends m1 m2 ->
-    cc_locset_ext_reply (lr ls1 m1) (lr ls2 m2).
+Inductive cc_locset_reply R w: locset_reply -> locset_reply -> Prop :=
+  cc_locset_reply_intro ls1 ls2 m1 m2:
+    (forall l, Val.inject (mi R w) (ls1 l) (ls2 l)) ->
+    match_mem R w m1 m2 ->
+    cc_locset_reply R w (lr ls1 m1) (lr ls2 m2).
 
-Program Definition cc_locset_ext :=
+Program Definition cc_locset R :=
   {|
-    ccworld := unit;
-    match_senv w := eq;
-    match_query w := cc_locset_ext_query;
-    match_reply w := cc_locset_ext_reply;
+    ccworld := world R;
+    match_senv := match_stbls R;
+    match_query := cc_locset_query R;
+    match_reply := (<> (cc_locset_reply R))%klr;
   |}.
+Next Obligation.
+  eapply match_stbls_proj in H. eapply Genv.mge_public; eauto.
+Qed.
+Next Obligation.
+  eapply match_stbls_proj in H. eapply Genv.valid_for_match; eauto.
+Qed.
