backend/Tunnelingproof.v
@@ -14,9 +14,10 @@
 
 Require Import Coqlib Maps UnionFind.
 Require Import AST Linking.
-Require Import Values Memory Events Globalenvs LanguageInterface Smallstep.
+Require Import Values Memory Events Globalenvs Smallstep.
 Require Import Op Locations Conventions LTL.
 Require Import Tunneling.
+Require Import LanguageInterface cklr.Extends.
 
 Definition match_prog (p tp: program) :=
   match_program (fun ctx f tf => tf = tunnel_fundef f) eq p tp.
@@ -522,38 +523,44 @@ Proof.
 Qed.
 
 Lemma transf_initial_states:
-  forall q1 q2 st1, cc_locset_ext_query q1 q2 -> initial_state ge q1 st1 ->
+  forall w q1 q2 st1, match_query (cc_locset ext) w q1 q2 -> initial_state ge q1 st1 ->
   exists st2, initial_state tge q2 st2 /\ match_states st1 st2.
 Proof.
-  intros. inv H. inv H0.
+  intros. inv H0. inv H. CKLR.uncklr. setoid_rewrite ext_lessdef in H7.
+  destruct H5 as [vf|]; try congruence.
   exists (Callstate (Stackbase ls2 :: nil) vf ls2 m2); split.
   - setoid_rewrite <- (sig_preserved (Internal f)).
-    eapply functions_translated in H7; eauto.
+    eapply functions_translated in H1; eauto.
     econstructor; eauto.
   - constructor; eauto.
     repeat constructor; eauto.
 Qed.
 
 Lemma transf_final_states:
-  forall st1 st2 r1, match_states st1 st2 -> final_state st1 r1 ->
-  exists r2, final_state st2 r2 /\ cc_locset_ext_reply r1 r2.
+  forall w st1 st2 r1, match_states st1 st2 -> final_state st1 r1 ->
+  exists r2, final_state st2 r2 /\ match_reply (cc_locset ext) w r1 r2.
 Proof.
   intros. inv H0. inv H. inv STK. inv H1.
-  exists (lr tls tm). split; constructor; auto.
+  exists (lr tls tm). split. constructor; auto.
+  exists tt. split; constructor; CKLR.uncklr; auto.
+  setoid_rewrite ext_lessdef; auto.
 Qed.
 
 Lemma transf_external_states:
   forall st1 st2 q1, match_states st1 st2 -> at_external ge st1 q1 ->
-  exists q2, at_external tge st2 q2 /\ cc_locset_ext_query q1 q2 /\ se = se /\
-  forall r1 r2 st1', cc_locset_ext_reply r1 r2 -> after_external st1 r1 st1' ->
+  exists q2, at_external tge st2 q2 /\ match_query (cc_locset ext) tt q1 q2 /\ se = se /\
+  forall r1 r2 st1', match_reply (cc_locset ext) tt r1 r2 -> after_external st1 r1 st1' ->
   exists st2', after_external st2 r2 st2' /\ match_states st1' st2'.
 Proof.
   intros. inv H0. inv H.
   exploit functions_translated; eauto. cbn. intros TFIND.
   eexists (lq tvf sg tls tm); intuition idtac.
   - econstructor; eauto.
-  - destruct LF; try discriminate. econstructor; eauto.
-  - inv H0. inv H.
+  - destruct LF; try discriminate. econstructor; CKLR.uncklr; eauto.
+    setoid_rewrite ext_lessdef. auto.
+    destruct v; cbn in *; try congruence.
+  - inv H0. destruct H as ([ ] & _ & H). inv H.
+    CKLR.uncklr. setoid_rewrite ext_lessdef in H3.
     eexists; split; econstructor; eauto.
 Qed.
 
@@ -561,10 +568,11 @@ End PRESERVATION.
 
 Theorem transf_program_correct prog tprog:
   match_prog prog tprog ->
-  forward_simulation cc_locset_ext cc_locset_ext (LTL.semantics prog) (LTL.semantics tprog).
+  forward_simulation (cc_locset ext) (cc_locset ext) (LTL.semantics prog) (LTL.semantics tprog).
 Proof.
   fsim eapply forward_simulation_opt; destruct Hse.
-  - intros q _ []. eapply (Genv.is_internal_transf_id MATCH). intros [|]; auto.
+  - intros q _ []. CKLR.uncklr. destruct H; try congruence.
+    eapply (Genv.is_internal_transf_id MATCH). intros [|]; auto.
   - eapply transf_initial_states; eauto.
   - eapply transf_final_states; eauto.
   - exists tt. eapply transf_external_states; eauto.
